\documentclass[journal,12pt,twocolumn]{IEEEtran}
\usepackage{amsmath,amssymb,amsfonts,amsthm}
\usepackage{txfonts}
\usepackage{tkz-euclide}
\usepackage{listings}
\usepackage{gvv}
\usepackage[latin1]{inputenc}
\usepackage{adjustbox}
\usepackage{array}
\usepackage{tabularx}
\usepackage{enumitem}
\usepackage{pgf}
\usepackage{lmodern}
\usepackage{circuitikz}
\usepackage{tikz}
\usepackage{graphicx}


\begin{document}
\bibliographystyle{IEEEtran}

\vspace{3cm}

\title{}
\author{EE23BTECH11054 -  Sai Krishna Shanigarapu$^{*}$
}
\maketitle
\newpage
\bigskip

% \renewcommand{\thefigure}{\theenumi}
% \renewcommand{\thetable}{\theenumi}

\section*{Gate ES 2022}
13. \hspace{2pt}Assuming $s>0$; Laplace transform for $f\brak{x}$ = $\sin\brak{ax}$ is\\
\begin{enumerate}[label=(\Alph*)]
    \item $\frac{a}{s^2+a^2}$\\
    \item $\frac{s}{s^2 + a^2}$\\
    \item $\frac{a}{s^2-a^2}$\\
    \item $\frac{s}{s^2-a^2}$
\end{enumerate}
\hfill(GATE 2022 ES)

\solution\\
Assuming $Re\brak{s}>0$\\
Using Table \ref{tab:tab1_2022_es_13_054}
\begin{enumerate}
    \item Proof 1: Using Definition\\
    \begin{align}
        \mathcal{L}\brak{\sin\brak{ax}} &= \int_{0}^{\infty}e^{-sx}\sin\brak{ax}\, dx\\
        &= \lim_{L\to \infty} \int_{0}^{L}e^{-sx}\sin\brak{ax}\, dx\\
      %  &= \lim_{L\to \infty}\sbrak{\frac{e^{-sx}\brak{-s\sin\brak{ax} - a\cos{ax}}}{\brak{-s}^2 + a^2}}_{0}^{L}\\
        &= \frac{s\sin\brak{0} + a\cos\brak{0}}{s^2 - a^2} - 0\\
        &= \frac{a}{s^2 + a^2}
    \end{align}
\bigskip
    \item Proof 2: Using Euler's identity\\
    \begin{align}
        \mathcal{L}\brak{\sin\brak{ax}} &= \mathcal{L}\brak{\frac{e^{jax} - e^{-jax}}{2j}}\\
        &= \frac{\brak{\mathcal{L}\brak{e^{jax}} - \mathcal{L}\brak{e^{-jax}}}}{2j}\\
        &= \frac{2}{2j}\brak{\frac{1}{s-ja}-\frac{1}{s+ja}}\\
        &= \frac{1}{2j}\brak{\frac{2ja}{s^2 + a^2}}\\
        &= \frac{a}{s^2 + a^2}
    \end{align}
\bigskip
    \item Proof 3: Using Laplace Transform of Second Derivative\\
    \begin{align}
        \mathcal{L}\brak{f''\brak{x}} &= s^2\mathcal{L}\brak{f\brak{x}} - sf\brak{0} - f'\brak{0}
    \end{align}
    Then ,
    \begin{align}
        f\brak{x} &= \sin\brak{ax}\\
        \implies f'\brak{x} &= a\cos\brak{ax}\\
        f''\brak{x} &= -a^2\, \sin\brak{ax}\\
        f\brak{0}&=0\\
        f'\brak{0} &= 0\\
        \implies \mathcal{L}\brak{-a^2\, \sin\brak{ax}} &= s^2\mathcal{L}\brak{\sin\brak{ax}} - a\\
       \implies -a^2\mathcal{L}\brak{\sin\brak{ax}} &= s^2\mathcal{L}\brak{\sin\brak{ax}} - a\\
       \implies \mathcal{L}\brak{\sin\brak{ax}} &= \frac{a}{s^2 + a^2}
    \end{align} 
\bigskip
    \item Proof 4: Using Laplace Transform of exponential\\
    \begin{align}
        \mathcal{L}\brak{e^{jax}} &= \mathcal{L}\brak{\cos\brak{ax} + j\sin\brak{ax}}\\
        &= \mathcal{L}\brak{\cos\brak{ax}} + j\mathcal{L}\brak{\sin\brak{ax}}\\
        \implies \mathcal{L}\brak{\sin\brak{ax}} &= \mathbf{Im}\brak{\mathcal{L}\brak{e^{jax}}}\\
        &= \mathbf{Im}\brak{\frac{s + ja}{s^2 + a^2}}\\
        &= \frac{a}{s^2 + a^2}
    \end{align}
\end{enumerate}
\bigskip

$\therefore$ Option (A) is correct.

\begin{table}[ht]
     \begin{adjustbox}{width=\columnwidth}
       \input{tables/table1}
    \end{adjustbox}
    \caption{Laplace transforms}
    \label{tab:tab1_2022_es_13_054}
\end{table}

\begin{figure}[ht]
    \centering
    \includegraphics[width=\columnwidth]{figs/Figure_1.png}
    \caption{plot of sin(ax) and it's laplace transform}
    \label{fig:fig1_2022_es_13_054}
\end{figure}

\begin{figure}[ht]
    \centering
    \includegraphics[width=\columnwidth]{figs/Figure_2.png}
    \caption{plots of laplace forms of sin(ax)}
    \label{fig:fig2_2022_es_13_054}
\end{figure}

\end{document}
